src/pki/mipki.h
@@ -2,6 +2,14 @@
 #define HEADER_MIPKIH
 #include <stdint.h>
 
+#if defined(_MSC_VER)  // Visual Studio - always use __cdecl keyword
+  #define MITLS_CALLCONV __cdecl
+#elif defined(__cdecl) // GCC/MinGW targeting Windows 32-bit - use the __cdecl macro
+  #define MITLS_CALLCONV __cdecl
+#else                  // Targeting other platforms - use the ambient calling convention
+  #define MITLS_CALLCONV
+#endif
+
 typedef struct {
   const char *cert_file;
   const char *key_file;
@@ -37,43 +45,43 @@ typedef const void* mipki_chain;
 
 // A callback used to ask for the passphrase of the private key
 // Should return the size of the written passphrase, or 0 on error
-typedef int (*password_callback)(char *pass, int max_size, const char *key_file);
+typedef int (MITLS_CALLCONV *password_callback)(char *pass, int max_size, const char *key_file);
 
 // Create a new instance of the PKI library using the provided server configuration
 // The configuration describes the selectable certificates as a server, and
 // their private keys. They are loaded in memory until mipki_free is called.
 // The created instance may be used in multiple TLS connections, for instance,
 // it is recommanded to share the mipki_state accoress incoming connections on a server
-mipki_state *mipki_init(const mipki_config_entry config[], size_t config_len, password_callback pcb, int *erridx);
-void mipki_free(mipki_state *st);
+mipki_state* MITLS_CALLCONV mipki_init(const mipki_config_entry config[], size_t config_len, password_callback pcb, int *erridx);
+void MITLS_CALLCONV mipki_free(mipki_state *st);
 
 // OpenSSL specific: configure a root certificate file or hash directory.
 // This is mandatory to perform certificate chain validation
-int mipki_add_root_file_or_path(mipki_state *st, const char *ca_file);
+int MITLS_CALLCONV mipki_add_root_file_or_path(mipki_state *st, const char *ca_file);
 
 // Find a certificate and signature algorithm compatible with the given SNI and list of offered signature algorithms
 // Returns a pointer to the selected entry or NULL if no certificate is suitable
-mipki_chain mipki_select_certificate(mipki_state *st, const char *sni, const mipki_signature *algs, size_t algs_len, mipki_signature *selected);
+mipki_chain MITLS_CALLCONV mipki_select_certificate(mipki_state *st, const char *sni, const mipki_signature *algs, size_t algs_len, mipki_signature *selected);
 
 // A combined signature-and-verify function (depending on m)
 // Returns 0 on error. When signing, pass a reference to the size of the signature buffer to sig_len,
 // after calling sig_len contains the acutal size of the signature. When verifying, pass a reference to the
 // input signature length.
-int mipki_sign_verify(mipki_state *st, mipki_chain cert_ptr, const mipki_signature sigalg, const char *tbs, size_t tbs_len, char *sig, size_t *sig_len, mipki_mode m);
+int MITLS_CALLCONV mipki_sign_verify(mipki_state *st, mipki_chain cert_ptr, const mipki_signature sigalg, const char *tbs, size_t tbs_len, char *sig, size_t *sig_len, mipki_mode m);
 
 // Parse a chain in TLS network format into an abstract chain object
 // Each certificate in the chain is encoded in DER, prefixed with the size of the
 // DER-encodeded structure over 3 bytes. The returned chain must be freed after use
-mipki_chain mipki_parse_chain(mipki_state *st, const char *chain, size_t chain_len);
+mipki_chain MITLS_CALLCONV mipki_parse_chain(mipki_state *st, const char *chain, size_t chain_len);
 
 // Format an abstract chain into the TLS network format
-size_t mipki_format_chain(mipki_state *st, mipki_chain chain, char *buffer, size_t buffer_len);
+size_t MITLS_CALLCONV mipki_format_chain(mipki_state *st, mipki_chain chain, char *buffer, size_t buffer_len);
 
 // Certificate chain validation. This checks revocation, expiration, and matches the hostname
-int mipki_validate_chain(mipki_state *st, mipki_chain chain, const char *host);
+int MITLS_CALLCONV mipki_validate_chain(mipki_state *st, mipki_chain chain, const char *host);
 
 // Free a chain after use.
-void mipki_free_chain(mipki_state *st, mipki_chain chain);
+void MITLS_CALLCONV mipki_free_chain(mipki_state *st, mipki_chain chain);
 
 
 #endif
